             -  <- 2^0 
     2^5 -> | | <- 2^1
      2^6 -> -
     2^4 -> | | <- 2^2
             - <- 2^3

0 -> 2^0 + 2^1 + 2^2 + 2^3 + 2^4 + 2^5        = 63
1 -> 2^1 + 2^2                                = 6
2 -> 2^0 + 2^1 + 2^6 + 2^4 + 2^3              = 91
3 -> 2^0 + 2^1 + 2^6 + 2^2 + 2^3              = 79
4 -> 2^5 + 2^6 + 2^1 + 2^2                    = 102
5 -> 2^0 + 2^5 + 2^6 + 2^2 + 2^3              = 109
6 -> 2^0 + 2^5 + 2^4 + 2^3 + 2^2 + 2^6        = 125
7 -> 2^0 + 2^1 + 2^2                          = 7
8 -> 2^0 + 2^1 + 2^2 + 2^3 + 2^4 + 2^5 + 2^6  = 127
9 -> 2^0 + 2^5 + 2^6 + 2^1 + 2^2 + 2^3        = 111
